\chapter{Pre-calculus results}

This chapter is made to provide a bunch of useful pre-calculus results.

\section{Algebra}
\subsection{Arithmetic Operations}

\[
  a(b + c) = ab + ac \hspace{5em}
  \frac{a + b}b = \frac ab + \frac cb \hspace{5em}
  \frac ab + \frac cd = \frac{ad + bc}{bd} \hspace{5em}
  \frac{\sfrac ab}{\sfrac cd} = \frac ab \times \frac dc = \frac{ad}{bc}
\]

\subsection{Exponents and Radicals}

\[
  x^m x^n = x^{m + n}\hspace{4em}
  (x^m)^n = x^{mn} \hspace{4em}
  (xy)^n = x^n y^n \hspace{4em}
  x^{\sfrac 1n} = \sqrt n \hspace{4em}
  \nthroot n{xy} = \nthroot nx \nthroot ny
\]

\[
  \frac{x^m}{x^n} = x^{m - n} \hspace{4em}
  x^{-1} = \frac 1{x^n} \hspace{4em}
  \parens*{\frac xy}^n = \frac{x^n}{y^n} \hspace{4em}
  x^{\sfrac mn} = \nthroot n{x^m} = \parens*{\nthroot nx}^m \hspace{4em}
  \nthroot n{\frac xy} = \frac{\nthroot nx}{\nthroot xy}
\]

\subsection{Factoring Special Polynomials}
\[
  x^2 - y^2 = (x + y) (x - y) \hspace{5em}
  x^3 + y^3 = (x + y) (x^2 - xy + y^2) \hspace{5em}
  x^3 - y^3 = (x - y) (x^2 + xy + y^2)
\]
\subsection{Binomial Theorem}

\[
  (x + y)^2 = x^2 + 2xy + y^2 \hspace{5em}
  (x - y)^2 = x^2 - 2xy + y^2 \hspace{5em}
\]

\[
  (x + y)^3 = x^3 + 3x^2y + 3xy^2 + y^3 \hspace{5em}
  (x - y)^3 = x^3 - 3x^2y + 3xy^2 - y^3 
\]
In general we have:
\[
  (x + y)^n = x^n + nx^{n-1}y + \frac{n(n-1)}2 x^{n-2}y^2 + \cdots + \binom nk x^{n-k}y^k + \cdots + nxy^{n-1} + y^n
\]

where

\begin{align*}
  \binom nk &= \frac{n!}{k! (n - k)!} \\
            &= \frac{n \cdot (n-1) \cdot (n-2) \cdot (n-3) \cdot \cdots \cdot 3 \cdot 2 \cdot 1}{k!(n - k)!}\\
            &= \frac{n \cdot (n-1) \cdot \cdots \cdot (n - k + 1) \cdot (n-k)!}{k!(n - k)!}\\
            &= \frac{n \cdot (n-1) \cdot \cdots \cdot (n - k + 1)}{k \cdot (k-1) \cdot (k-2) \cdot \cdots \cdot 2 \cdot 1}
\end{align*}

\subsection{Quadratic Formula}
